Prove up through let case of sub lemma
Define conversions to sets
Define free vars, prove equivalent to core free vars under eval
Add to typing rules and complete let case
Prove inversion lemmas for rest of cases
Prove alt pattern ind principle

src/proofs/ElimLet/BindingProofs.v
@@ -292,6 +292,62 @@ Proof.
   bool_hyps. apply t_similar_ty; auto.
 Qed.
 
+(*TODO: move this stuff*)
+
+(*Ignore ocurrence count*)
+
+Fixpoint p_free_vars (p: pattern_c) : Svs.t :=
+  match pat_node_of p with
+  | TermDefs.Pvar v => Svs.singleton v
+  | Papp l ps => fold_right Svs.union Svs.empty (map p_free_vars ps)
+  | TermDefs.Por p1 p2 => Svs.union (p_free_vars p1) (p_free_vars p2)
+  | Pas p v => Svs.union (p_free_vars p) (Svs.singleton v)
+  | TermDefs.Pwild => Svs.empty
+  end.
+
+Fixpoint t_free_vars (t: term_c) : Svs.t :=
+  match t_node_of t with
+  | TermDefs.Tvar v => Svs.singleton v
+  | TermDefs.Tlet t1 (v, _, t2) => Svs.union (t_free_vars t1) (Svs.remove v (t_free_vars t2))
+  | TermDefs.Tif t1 t2 t3 => Svs.union (t_free_vars t1) (Svs.union (t_free_vars t2) (t_free_vars t3))
+  | Tapp l tms => (fold_right Svs.union Svs.empty (map t_free_vars tms))
+  | Tcase t1 ps => Svs.union (t_free_vars t1) (fold_right Svs.union Svs.empty
+      (map (fun x => Svs.diff (t_free_vars (snd x)) (p_free_vars (fst (fst x)))) ps) )
+  | TermDefs.Teps (v, _, t) => Svs.remove v (t_free_vars t)
+  | Tquant _ (vs, _, _, t) => Svs.diff (t_free_vars t) (Svs.of_list vs)
+  | Tbinop _ t1 t2 => Svs.union (t_free_vars t1) (t_free_vars t2)
+  | Tnot t1 => t_free_vars t1
+  | _ => Svs.empty
+  end.
+
+(*rewrite lemmas*)
+Lemma p_free_vars_rewrite p:
+  p_free_vars p =
+  match pat_node_of p with
+  | TermDefs.Pvar v => Svs.singleton v
+  | Papp l ps => fold_right Svs.union Svs.empty (map p_free_vars ps)
+  | TermDefs.Por p1 p2 => Svs.union (p_free_vars p1) (p_free_vars p2)
+  | Pas p v => Svs.union (p_free_vars p) (Svs.singleton v)
+  | TermDefs.Pwild => Svs.empty
+  end.
+Proof. destruct p; auto. Qed.
+
+Lemma t_free_vars_rewrite t:
+  t_free_vars t = match t_node_of t with
+  | TermDefs.Tvar v => Svs.singleton v
+  | TermDefs.Tlet t1 (v, _, t2) => Svs.union (t_free_vars t1) (Svs.remove v (t_free_vars t2))
+  | TermDefs.Tif t1 t2 t3 => Svs.union (t_free_vars t1) (Svs.union (t_free_vars t2) (t_free_vars t3))
+  | Tapp l tms => (fold_right Svs.union Svs.empty (map t_free_vars tms))
+  | Tcase t1 ps => Svs.union (t_free_vars t1) (fold_right Svs.union Svs.empty
+      (map (fun x => Svs.diff (t_free_vars (snd x)) (p_free_vars (fst (fst x)))) ps) )
+  | TermDefs.Teps (v, _, t) => Svs.remove v (t_free_vars t)
+  | Tquant _ (vs, _, _, t) => Svs.diff (t_free_vars t) (Svs.of_list vs)
+  | Tbinop _ t1 t2 => Svs.union (t_free_vars t1) (t_free_vars t2)
+  | Tnot t1 => t_free_vars t1
+  | _ => Svs.empty
+  end.
+Proof. destruct t; auto. Qed.
+
 (*Need predicate that types are consistent - this is not a full type system*)
 Fixpoint types_wf (t: term_c) : Prop :=
   match t_node_of t with
@@ -299,7 +355,8 @@ Fixpoint types_wf (t: term_c) : Prop :=
   | Tconst _ => True
   | Tapp l tms => (*TODO: need anything else?*)  Forall (fun x => x) (map types_wf tms)
   | Tif t1 t2 t3 => t_ty_of t2 = t_ty_of t3 /\ t_ty_of t2 = t_ty_of t /\ types_wf t1 /\ types_wf t2 /\ types_wf t3
-  | Tlet t1 (v, _, t2) => (*t_ty_of t1 = Some (vs_ty v) /\ t_ty_of t2 = t_ty_of t /\*) types_wf t1 /\ types_wf t2
+  | Tlet t1 (v, b, t2) => Mvs.map (fun _ => tt) (bv_vars b) = t_free_vars t2 /\
+     (*t_ty_of t1 = Some (vs_ty v) /\ t_ty_of t2 = t_ty_of t /\*) types_wf t1 /\ types_wf t2
   | Tcase t1 ps => (*TODO: see*) types_wf t1 /\ 
       Forall (fun x => x) (map (fun x => types_wf (snd x)) ps) (*see if we need more*)
      (*  Forall (fun x => x) (map (fun x => t_ty_of t1 = Some (pat_ty_of (fst (fst x))) /\
@@ -317,7 +374,7 @@ Lemma types_wf_rewrite t:
   | Tconst _ => True
   | Tapp l tms => (*TODO: need anything else?*) Forall (fun x => x) (map types_wf tms)
   | Tif t1 t2 t3 => t_ty_of t2 = t_ty_of t3 /\ t_ty_of t2 = t_ty_of t /\ types_wf t1 /\ types_wf t2 /\ types_wf t3
-  | Tlet t1 (v, _, t2) => (*t_ty_of t1 = Some (vs_ty v) /\ t_ty_of t2 = t_ty_of t /\*) types_wf t1 /\ types_wf t2
+  | Tlet t1 (v, b, t2) =>  Mvs.map (fun _ => tt) (bv_vars b) = t_free_vars t2 /\ (*t_ty_of t1 = Some (vs_ty v) /\ t_ty_of t2 = t_ty_of t /\*) types_wf t1 /\ types_wf t2
   | Tcase t1 ps => types_wf t1 /\ 
       Forall (fun x => x) (map (fun x => types_wf (snd x)) ps)
   | Teps (v, _, t1) => types_wf t1
@@ -1870,6 +1927,478 @@ Proof.
   apply vsymbol_eqb_eq in Heq. subst. apply Hall. destruct x; auto.
 Qed.
 
+Print term_c.
+Print tm_fv.
+
+
+(*We have 3 things to do
+  1. Define function Mvs.t A -> Svs.t (just a map really) and prove how it commutes with
+    (eval_var_set)
+  2. Add this to typing rules
+  3. Prove that these correspond to pat_fv, tm_fv, and fmla_fv in eval*)
+
+(*Start with last one*)
+
+(*Eval Svs.t*)
+(* Definition eval_svs (s: Svs.t) : aset vsymbol :=
+  eval_varset s. *)
+
+(*Pattern first*)
+
+(*Alt ind principle*)
+Section PatternIndAlt.
+
+Variable (P: pattern_c -> Prop).
+
+Variable (Hvar: forall v p (Heq: pat_node_of p = TermDefs.Pvar v), P p).
+Variable (Happ: forall l ps p (Heq: pat_node_of p = Papp l ps), Forall P ps -> P p).
+Variable (Hor: forall p1 p2 p (Heq: pat_node_of p = TermDefs.Por p1 p2), P p1 -> P p2 -> P p).
+Variable (Has: forall p1 v p (Heq: pat_node_of p = TermDefs.Pas p1 v), P p1 -> P p).
+Variable (Hwild: forall p (Heq: pat_node_of p = TermDefs.Pwild), P p).
+
+
+Fixpoint pat_ind_alt (p: pattern_c) : P p :=
+  match pat_node_of p as p1 return pat_node_of p = p1 -> P p with
+  | TermDefs.Pvar v => Hvar v p
+  | TermDefs.Papp l ps => fun Heq => Happ l ps p Heq (mk_Forall pat_ind_alt ps)
+  | TermDefs.Por p1 p2 => fun Heq => Hor p1 p2 p Heq (pat_ind_alt p1) (pat_ind_alt p2)
+  | TermDefs.Pas p1 v => fun Heq => Has p1 v p Heq (pat_ind_alt p1)
+  | TermDefs.Pwild => Hwild p
+  end eq_refl.
+
+End PatternIndAlt.
+
+(*Inversion lemmas - TODO move*)
+
+Ltac destruct_pat_node p :=
+  let n := fresh "n" in
+  destruct p as [n ? ?]; destruct n; try discriminate; simpl in *; subst; simpl in *.
+
+Lemma eval_pat_tm {p e v} 
+  (Hn: pat_node_of p = TermDefs.Pvar v)
+  (Heval: eval_pat p = Some e):
+  e = Pvar (eval_vsymbol v).
+Proof.
+  destruct_pat_node p. inversion Hn; subst. inversion Heval; subst; auto.
+Qed.
+
+Lemma eval_pat_app {p l ps e} (Hn: pat_node_of p = TermDefs.Papp l ps)
+  (Heval: eval_pat p = Some e):
+  exists l1 (*tys'*) tys1 ps1,
+    e = Pconstr l1 tys1 ps1 /\ eval_funsym l = Some l1 /\
+      (*fold_list_option (map pat_type ps) = Some tys' /\*)
+      funpred_ty_list l1 (map pat_type ps) = Some tys1 /\
+      fold_list_option (map eval_pat ps) = Some ps1.
+Proof.
+  destruct_pat_node p. inversion Hn; subst. apply option_bind_some in Heval.
+  destruct Heval as [l1 [Heval Hbind]]. apply option_bind_some in Hbind.
+  destruct Hbind as [ps1 [Hps Hbind]]. apply option_map_some in Hbind.
+  destruct Hbind as [tys1 [Htys He]]; subst.
+  exists l1. exists tys1. exists ps1. auto.
+Qed.
+
+Lemma eval_pat_or {p p1 p2 e} (Hn: pat_node_of p = TermDefs.Por p1 p2)
+  (Heval: eval_pat p = Some e):
+  exists e1 e2, e = Por e1 e2 /\ eval_pat p1 = Some e1 /\ eval_pat p2 = Some e2.
+Proof.
+  destruct_pat_node p. inversion Hn; subst. apply option_bind_some in Heval.
+  destruct Heval as [e1 [Heval1 Hbind]]. apply option_bind_some in Hbind.
+  destruct Hbind as [e2 [Heval2 Hbind]]. inversion Hbind; subst.
+  eauto.
+Qed.
+
+Lemma eval_pat_as {p p1 v e} (Hn: pat_node_of p = TermDefs.Pas p1 v)
+  (Heval: eval_pat p = Some e):
+  exists p1', e = Pbind p1' (eval_vsymbol v) /\ eval_pat p1 = Some p1'.
+Proof.
+  destruct_pat_node p. inversion Hn; subst. apply option_bind_some in Heval. 
+  destruct Heval as [p1' [Heval Hsome]]. inversion Hsome; subst.
+  exists p1'; auto.
+Qed.
+
+Lemma eval_pat_wild {p e} (Hn: pat_node_of p = TermDefs.Pwild) (Heval: eval_pat p = Some e):
+  e = Pwild.
+Proof.
+  destruct_pat_node p. inversion Heval; auto.
+Qed.
+
+(*TODO: move with others*)
+Check Mvs.singleton.
+Lemma eval_varset_singleton {A: Type} x y:
+  @eval_varset A (Mvs.singleton _ x y) = aset_singleton (eval_vsymbol x).
+Proof.
+  apply aset_ext. intros z. simpl_set.
+  rewrite eval_varset_mem. split.
+  - intros [y1 [Hz Hiny]]; subst.
+    rewrite Mvs.mem_spec, Mvs.singleton_spec in Hiny; auto.
+    destruct (Vsym.Tg.equal y1 x) eqn : Heq; try discriminate.
+    apply vsymbol_eqb_eq in Heq. subst; auto.
+  - intros Hz; subst. exists x. split; auto.
+    rewrite Mvs.mem_spec, Mvs.singleton_spec; auto.
+    rewrite Vsym.Tg.eq_refl. auto.
+Qed.
+
+Lemma eval_varset_union (s1 s2: Svs.t):
+  eval_varset (Svs.union s1 s2) = aset_union (eval_varset s1) (eval_varset s2).
+Proof.
+  apply aset_ext. intros x. simpl_set.
+  rewrite !eval_varset_mem. setoid_rewrite Mvs.mem_spec. 
+  unfold Svs.union. setoid_rewrite Mvs.set_union_spec.
+  split.
+  - intros [y [Hxy Hmemy]]; subst. destruct (Mvs.find_opt y s1) eqn : Hfind1.
+    + left. exists y. rewrite Hfind1. auto.
+    + destruct (Mvs.find_opt y s2) eqn : Hfind2; [|discriminate].
+      right. exists y. rewrite Hfind2. auto.
+  - intros [[y [Hxy Hsome]] | [y [Hxy Hsome]]]; subst; exists y; split; auto;
+    destruct (Mvs.find_opt y s1); auto.
+Qed.
+
+Lemma eval_varset_big_union {A} (f: A -> Svs.t)(l: list A):
+  eval_varset (fold_right Svs.union Svs.empty (map f l)) =
+  aset_big_union (fun x => eval_varset (f x)) l.
+Proof.
+  induction l as [| h t IH]; simpl; auto.
+  rewrite eval_varset_union, IH. reflexivity.
+Qed. 
+
+Lemma eval_varset_empty {A}:
+  @eval_varset A Mvs.empty = aset_empty.
+Proof.
+  apply aset_ext. intros x.
+  rewrite eval_varset_mem.
+  split.
+  - intros [y [Hx Hmemy]]. subst.
+    rewrite Mvs.mem_spec, Mvs.empty_spec in Hmemy. discriminate.
+  - intros Hmem. simpl_set.
+Qed.
+
+Print Svs.remove.
+Print Mvs.remove.
+Lemma eval_varset_remove {A} (m: Mvs.t A) k:
+  eval_varset (Mvs.remove _ k m) = aset_remove (eval_vsymbol k) (eval_varset m).
+Proof.
+  apply aset_ext. intros x. simpl_set. rewrite !eval_varset_mem. setoid_rewrite Mvs.mem_spec.
+  setoid_rewrite Mvs.remove_spec. split.
+  - intros [y [Hx Heq]]. subst. 
+    destruct (Vsym.Tg.equal y k) eqn : Heq'; try discriminate.
+    split; eauto. intros Hc. apply eval_vsymbol_inj in Hc. subst. rewrite Vsym.Tg.eq_refl in Heq'.
+    discriminate.
+  - intros [[y [Hx Hsome]] Hnotx]; subst.
+    exists y. split; auto. destruct (Vsym.Tg.equal y k) eqn : Heq; auto.
+    apply vsymbol_eqb_eq in Heq. subst. contradiction.
+Qed.
+
+Lemma eval_varset_diff {A B} (m1: Mvs.t A) (m2: Mvs.t B):
+  eval_varset (Mvs.set_diff _ _ m1 m2) = aset_diff (eval_varset m2) (eval_varset m1).
+Proof.
+  apply aset_ext. intros x. simpl_set. rewrite !eval_varset_mem. setoid_rewrite Mvs.mem_spec.
+  setoid_rewrite Mvs.set_diff_spec. split.
+  - intros [y [Hx Heq]]. subst.
+    destruct (Mvs.find_opt y m1) eqn : Hfind1; try discriminate.
+    destruct (Mvs.find_opt y m2) eqn : Hfin2; try discriminate.
+    split.
+    + exists y. rewrite Hfind1. auto.
+    + intros [y1 [Heqy Hsome]]. apply eval_vsymbol_inj in Heqy. subst.
+      rewrite Hfin2 in Hsome. discriminate.
+  - intros [[y [Hx Hsome]] Hnotex]. subst. exists y. split; auto. 
+    destruct (Mvs.find_opt y m1) eqn : Hget1; try discriminate.
+    destruct (Mvs.find_opt y m2) eqn : Hget2; auto.
+    exfalso; apply Hnotex. exists y. rewrite Hget2. auto.
+Qed.
+
+Lemma p_free_vars_eval (p: pattern_c) (e: pattern) (Heval: eval_pat p = Some e):
+  eval_varset (p_free_vars p) = pat_fv e.
+Proof.
+  generalize dependent e.
+  induction p using pat_ind_alt; simpl; auto; intros e Heval; rewrite p_free_vars_rewrite, Heq.
+  - rewrite (eval_pat_tm Heq Heval); simpl.
+    apply eval_varset_singleton.
+  - rewrite eval_varset_big_union.
+    destruct (eval_pat_app Heq Heval) as [l1 [tys1 [ps2 [He [Hl [Htys1 Hps1]]]]]]; subst.
+    simpl. clear -H Hps1. generalize dependent ps2. induction ps as [| p1 t1 IH]; simpl.
+    + intros [| p2 t2]; try discriminate. auto.
+    + inversion H as [| ? ? Heq1 Heq2]; subst; clear H.
+      intros ps2 Hbind. apply option_bind_some in Hbind. destruct Hbind as [p2 [Heval1 Hbind]].
+      apply option_bind_some in Hbind. destruct Hbind as [t2 [Hopt Hsome]]. inversion Hsome; subst.
+      simpl. rewrite (Heq1 _ Heval1). f_equal. auto.
+  - rewrite eval_varset_union. destruct (eval_pat_or Heq Heval) as [e1 [e2 [He [Heval1 Heval2]]]].
+    subst. rewrite (IHp1 _ Heval1), (IHp2 _ Heval2); auto.
+  - destruct (eval_pat_as Heq Heval) as [e1 [He Heval1]]. subst. simpl.
+    rewrite eval_varset_union, (IHp1 _ Heval1). f_equal. apply eval_varset_singleton.
+  - rewrite (eval_pat_wild Heq Heval). simpl. apply eval_varset_empty.
+Qed.
+
+(*TODO: should use option_map not bind but whatever*)
+Lemma eval_match_tm {f1 t ps g1} (Hn: t_node_of f1 = Tcase t ps)
+  (Heval: eval_term f1 = Some g1):
+  exists t1 ty1 ps1, g1 = Tmatch t1 ty1 ps1 /\ eval_term t = Some t1 /\
+    term_type t = Some ty1 /\ fold_list_option (map (fun x => option_bind (eval_pat (fst (fst x)))
+      (fun p => option_bind (eval_term (snd x)) (fun t' => Some (p, t')))) ps) = Some ps1.
+Proof.
+  destruct_term_node f1. inversion Hn; subst; auto.
+  apply option_bind_some in Heval. destruct Heval as [e1 [Heval1 Hbind]].
+  apply option_bind_some in Hbind. destruct Hbind as [ty1 [Hty1 Hbind]].
+  apply option_bind_some in Hbind. destruct Hbind as [ps1 [Hfold Hsome]].
+  inversion Hsome; subst. eauto 10.
+Qed.
+
+Lemma eval_match_fmla {f1 t ps g1} (Hn: t_node_of f1 = Tcase t ps)
+  (Heval: eval_fmla f1 = Some g1):
+  exists t1 ty1 ps1, g1 = Fmatch t1 ty1 ps1 /\ eval_term t = Some t1 /\
+    term_type t = Some ty1 /\ fold_list_option (map (fun x => option_bind (eval_pat (fst (fst x)))
+      (fun p => option_bind (eval_fmla (snd x)) (fun t' => Some (p, t')))) ps) = Some ps1.
+Proof.
+  destruct_term_node f1. inversion Hn; subst; auto.
+  apply option_bind_some in Heval. destruct Heval as [e1 [Heval1 Hbind]].
+  apply option_bind_some in Hbind. destruct Hbind as [ty1 [Hty1 Hbind]].
+  apply option_bind_some in Hbind. destruct Hbind as [ps1 [Hfold Hsome]].
+  inversion Hsome; subst. eauto 10.
+Qed.
+
+Lemma eval_eps_tm {f1 tb g1} (Hn: t_node_of f1 = TermDefs.Teps tb)
+  (Heval: eval_term f1 = Some g1):
+  exists g2, g1 = Teps g2 (eval_vsymbol (fst (fst tb))) /\ eval_fmla (snd tb) = Some g2.
+Proof.
+  destruct_term_node f1. inversion Hn; subst. destruct tb as [[v1 b1] t1]; simpl in *.
+  apply option_bind_some in Heval. destruct Heval as [g2 [Heval Hsome]]; inversion Hsome; subst.
+  eauto.
+Qed.
+
+Lemma eval_eps_fmla {f1 tb g1} (Hn: t_node_of f1 = TermDefs.Teps tb)
+  (Heval: eval_fmla f1 = Some g1):
+  False.
+Proof.
+  destruct_term_node f1.
+Qed.
+
+Lemma eval_quant_fmla {f1 q tq g1} (Hn: t_node_of f1 = Tquant q tq)
+  (Heval: eval_fmla f1 = Some g1):
+  exists g2, g1 = (match q with | TermDefs.Tforall => fforalls | TermDefs.Texists => fexists end) 
+    (map eval_vsymbol (fst (fst (fst tq)))) g2 /\
+    eval_fmla (snd tq) = Some g2.
+Proof.
+  destruct_term_node f1. inversion Hn; subst. destruct tq as [[[vs b] tr] f].
+  simpl. apply option_bind_some in Heval. destruct Heval as [e1 [Heval1 Hsome]].
+  inversion Hsome; subst. destruct q; eauto.
+Qed.
+
+Lemma eval_quant_tm {f1 q tq g1} (Hn: t_node_of f1 = Tquant q tq)
+  (Heval: eval_term f1 = Some g1):
+  False.
+Proof.
+  destruct_term_node f1.
+Qed.
+
+Lemma eval_binop_fmla {f1 b t1 t2 g1} (Hn: t_node_of f1 = TermDefs.Tbinop b t1 t2)
+  (Heval: eval_fmla f1 = Some g1):
+  exists e1 e2, g1 = Fbinop (eval_binop b) e1 e2 /\ eval_fmla t1 = Some e1 /\ eval_fmla t2 = Some e2.
+Proof.
+  destruct_term_node f1. inversion Hn; subst. apply option_bind_some in Heval.
+  destruct Heval as [e1 [He1 Hbind]]. apply option_bind_some in Hbind. destruct Hbind as [e2 [He2 Hsome]].
+  inversion Hsome; subst. eauto.
+Qed.
+
+Lemma eval_binop_tm {f1 b t1 t2 g1} (Hn: t_node_of f1 = TermDefs.Tbinop b t1 t2)
+  (Heval: eval_term f1 = Some g1):
+  False.
+Proof. destruct_term_node f1. Qed.
+
+Lemma eval_not_fmla {f1 f2 g1} (Hn: t_node_of f1 = TermDefs.Tnot f2) (Heval: eval_fmla f1 = Some g1):
+  exists g2, g1 = Fnot g2 /\ eval_fmla f2 = Some g2.
+Proof.
+  destruct_term_node f1. inversion Hn; subst. apply option_bind_some in Heval.
+  destruct Heval as [g2 [Heval1 Hsome]]; inversion Hsome; eauto.
+Qed.
+
+Lemma eval_not_tm {f1 f2 g1} (Hn: t_node_of f1 = TermDefs.Tnot f2) (Heval: eval_term f1 = Some g1):
+  False.
+Proof. destruct_term_node f1. Qed.
+
+Lemma eval_true_fmla {f1 g1} (Hn: t_node_of f1 = TermDefs.Ttrue) (Heval: eval_fmla f1 = Some g1):
+  g1 = Ftrue.
+Proof.
+  destruct_term_node f1. inversion Heval; auto.
+Qed.
+
+Lemma eval_false_fmla {f1 g1} (Hn: t_node_of f1 = TermDefs.Tfalse) (Heval: eval_fmla f1 = Some g1):
+  g1 = Ffalse.
+Proof.
+  destruct_term_node f1. inversion Heval; auto.
+Qed.
+
+Lemma eval_true_tm {f1 g1} (Hn: t_node_of f1 = TermDefs.Ttrue) (Heval: eval_term f1 = Some g1):
+  False.
+Proof. destruct_term_node f1. Qed.
+
+Lemma eval_false_tm {f1 g1} (Hn: t_node_of f1 = TermDefs.Tfalse) (Heval: eval_term f1 = Some g1):
+  False.
+Proof. destruct_term_node f1. Qed.
+
+
+
+(*TODO: copied from [eliminate_algebraic_typing]; MOVE!*)
+
+Lemma fmla_fv_fforalls (vs: list vsymbol) (f: formula):
+  fmla_fv (fforalls vs f) = aset_diff (list_to_aset vs) (fmla_fv f).
+Proof.
+  induction vs as [| v vs IH]; simpl; auto.
+  - rewrite list_to_aset_nil, aset_diff_empty. reflexivity.
+  - rewrite IH. rewrite list_to_aset_cons.
+    apply aset_ext. intros x. simpl_set. 
+    split; intros; destruct_all; subst; split; auto.
+    intros [Hxv | Hinx]; subst; contradiction.
+Qed.
+
+Lemma fmla_fv_fexists (vs: list vsymbol) (f: formula):
+  fmla_fv (fexists vs f) = aset_diff (list_to_aset vs) (fmla_fv f).
+Proof.
+  induction vs as [| v vs IH]; simpl; auto.
+  - rewrite list_to_aset_nil, aset_diff_empty. reflexivity.
+  - rewrite IH. rewrite list_to_aset_cons.
+    apply aset_ext. intros x. simpl_set. 
+    split; intros; destruct_all; subst; split; auto.
+    intros [Hxv | Hinx]; subst; contradiction.
+Qed.
+
+Lemma eval_varset_add {A: Type} (m: Mvs.t A) x y:
+  eval_varset (Mvs.add x y m) = aset_union (aset_singleton (eval_vsymbol x)) (eval_varset m).
+Proof.
+  apply aset_ext. intros z. simpl_set. rewrite !eval_varset_mem.
+  setoid_rewrite Mvs.mem_spec. setoid_rewrite Mvs.add_spec.
+  split.
+  - intros [y1 [Hzy Hsome]]. subst. destruct ( Vsym.Tg.equal y1 x) eqn : Heq.
+    + apply vsymbol_eqb_eq in Heq; subst. auto.
+    + right. exists y1. auto.
+  - intros [Hz | [y1 [Hz Hsome]]]; subst; eauto.
+    + exists x. split; auto. rewrite Vsym.Tg.eq_refl. auto.
+    + exists y1. split; auto. destruct (Vsym.Tg.equal y1 x) eqn : Heq; auto.
+Qed.
+
+Lemma eval_varset_of_list l:
+  eval_varset (Svs.of_list l) = list_to_aset (map eval_vsymbol l).
+Proof.
+  induction l as [| h t IH ]; simpl; auto. unfold Svs.add.
+  rewrite list_to_aset_cons, eval_varset_add, IH. reflexivity.
+Qed.
+
+(*And for terms*)
+Lemma t_free_vars_eval (t: term_c):
+  (forall e (Heval: eval_term t = Some e), eval_varset (t_free_vars t) = tm_fv e) /\
+  (forall e (Heval: eval_fmla t = Some e), eval_varset (t_free_vars t) = fmla_fv e).
+Proof.
+  induction t using term_ind_alt; split; intros e Heval; rewrite t_free_vars_rewrite; try rewrite Heq; try rewrite Ht.
+  - (*Tvar*) rewrite (eval_var_tm Heq Heval). simpl. apply eval_varset_singleton.
+  - (*Fvar*) exfalso. apply (eval_var_fmla Heq Heval).
+  - (*Tconst*) destruct (eval_const_tm Heq Heval) as [c1 [He Hc1]]; subst.
+      simpl. apply eval_varset_empty.
+  - (*Fconst*) exfalso. apply (eval_const_fmla Heq Heval).
+  - (*Tfun*) destruct (eval_app_tm Heq Heval) as [l1 [tys' [tys1 [ts1 [He1 [Hevall [Htys [Htys1 Hts]]]]]]]]; subst.
+    simpl. rewrite eval_varset_big_union. clear -Hts H. generalize dependent ts1.
+    induction ts as [| t1 tl1 IH]; simpl; auto.
+    + intros [| t2 tl2]; try discriminate. auto.
+    + inversion H as [| ? ? [Heq1 _] Heq2]; subst; clear H.
+      intros ts1 Hbind. apply option_bind_some in Hbind. destruct Hbind as [t2 [Heval1 Hbind]].
+      apply option_bind_some in Hbind. destruct Hbind as [tl2 [Hopt Hsome]]. inversion Hsome; subst.
+      simpl. rewrite (Heq1 _ Heval1). f_equal. auto.
+  - destruct (eval_app_fmla Heq Heval) as [[Hl [t1' [t2' [t3' [t4' [ty1 [Hts [He1 [Ht1' [Ht2' Hty]]]]]]]]]] | 
+      [Hl [fs [tys [ty1 [tms [He1 [Hfs [Htys [Htys1 Htms]]]]]]]]]]; subst.
+    + (*Feq*) simpl. rewrite !eval_varset_union.
+      assert (Hemp: (eval_varset Svs.empty) = aset_empty) by (apply eval_varset_empty). rewrite Hemp, aset_union_empty_r.
+      inversion H as [| ? ? [IH1 _] Hrest]; subst. inversion Hrest as [| ? ? [IH2 _] _]; subst; clear H Hrest.
+      f_equal; auto.
+    + (*Fpred*) simpl. rewrite eval_varset_big_union. clear -Htms H. generalize dependent tms.
+      induction ts as [| t1 tl1 IH]; simpl; auto.
+      * intros [| t2 tl2]; try discriminate. auto.
+      * inversion H as [| ? ? [Heq1 _] Heq2]; subst; clear H.
+        intros ts1 Hbind. apply option_bind_some in Hbind. destruct Hbind as [t2 [Heval1 Hbind]].
+        apply option_bind_some in Hbind. destruct Hbind as [tl2 [Hopt Hsome]]. inversion Hsome; subst.
+        simpl. rewrite (Heq1 _ Heval1). f_equal. auto.
+  - (*Tif*) rewrite !eval_varset_union. destruct (eval_if_tm Heq Heval) as [e1 [e2 [e3 [He [He1 [He2 He3]]]]]]; subst.
+     simpl. destruct_all. f_equal; auto. f_equal; auto.
+  - (*Fif*) rewrite !eval_varset_union. destruct (eval_if_fmla Heq Heval) as [e1 [e2 [e3 [He [He1 [He2 He3]]]]]]; subst.
+    simpl. destruct_all. f_equal; auto. f_equal; auto.
+  - (*Tlet*) destruct (eval_let_tm Heq Heval) as [e1 [e2 [He [He1 He2]]]]. subst. simpl in *.
+    destruct IHt1 as [IH1 _]. destruct IHt2 as [IH2 _]. unfold Svs.remove.
+    rewrite !eval_varset_union, (IH1 _ He1), eval_varset_remove, (IH2 _ He2). reflexivity.
+  - (*Flet*) destruct (eval_let_fmla Heq Heval) as [e1 [e2 [He [He1 He2]]]]. subst. simpl in *.
+    destruct IHt1 as [IH1 _]. destruct IHt2 as [_ IH2]. unfold Svs.remove.
+    rewrite !eval_varset_union, (IH1 _ He1), eval_varset_remove, (IH2 _ He2). reflexivity.
+  - (*Tmatch*) destruct (eval_match_tm Heq Heval) as [e1 [ty1 [ps1 [He [He1 [Hty1 Hps1]]]]]].
+    subst. simpl. rewrite eval_varset_union. destruct IHt1 as [IH1 _]. rewrite (IH1 _ He1).
+    f_equal. rewrite eval_varset_big_union. rewrite Forall_map in H. clear -Hps1 H.
+    generalize dependent ps1. induction tbs as [| [[p1 b1] t1] tl1 IH]; simpl; auto.
+    + intros [| ? ?]; try discriminate; auto.
+    + intros ps1 Hbind. apply option_bind_some in Hbind. destruct Hbind as [pt [Hbind1 Hbind2]].
+      apply option_bind_some in Hbind1. destruct Hbind1 as [p2 [Hevalp Hbind1]].
+      apply option_bind_some in Hbind1. destruct Hbind1 as [t2 [Hevalt Hsome]]. inversion Hsome; subst; clear Hsome.
+      apply option_bind_some in Hbind2. destruct Hbind2 as [tl2 [Hfold Hsome]]. inversion Hsome; subst; clear Hsome.
+      simpl. inversion H as [| ? ? [IH1 _] IH2]; subst; clear H. simpl in *.
+      unfold Svs.diff. rewrite eval_varset_diff, (p_free_vars_eval _ _ Hevalp), (IH1 _ Hevalt). f_equal. auto.
+  - (*Fmatch*) destruct (eval_match_fmla Heq Heval) as [e1 [ty1 [ps1 [He [He1 [Hty1 Hps1]]]]]].
+    subst. simpl. rewrite eval_varset_union. destruct IHt1 as [IH1 _]. rewrite (IH1 _ He1).
+    f_equal. rewrite eval_varset_big_union. rewrite Forall_map in H. clear -Hps1 H.
+    generalize dependent ps1. induction tbs as [| [[p1 b1] t1] tl1 IH]; simpl; auto.
+    + intros [| ? ?]; try discriminate; auto.
+    + intros ps1 Hbind. apply option_bind_some in Hbind. destruct Hbind as [pt [Hbind1 Hbind2]].
+      apply option_bind_some in Hbind1. destruct Hbind1 as [p2 [Hevalp Hbind1]].
+      apply option_bind_some in Hbind1. destruct Hbind1 as [t2 [Hevalt Hsome]]. inversion Hsome; subst; clear Hsome.
+      apply option_bind_some in Hbind2. destruct Hbind2 as [tl2 [Hfold Hsome]]. inversion Hsome; subst; clear Hsome.
+      simpl. inversion H as [| ? ? [_ IH1] IH2]; subst; clear H. simpl in *.
+      unfold Svs.diff. rewrite eval_varset_diff, (p_free_vars_eval _ _ Hevalp), (IH1 _ Hevalt). f_equal. auto.
+  - (*Teps*) destruct (eval_eps_tm Heq Heval) as [e1 [He He1]]. simpl in *; subst.
+    simpl. unfold Svs.remove. rewrite eval_varset_remove. f_equal. destruct_all; auto.
+  - (*Feps*) exfalso. apply (eval_eps_fmla Heq Heval).
+  - (*Tquant*) exfalso. apply (eval_quant_tm Heq Heval).
+  - (*Fquant*) destruct (eval_quant_fmla Heq Heval) as [e1 [He He1]]. simpl in *. subst. unfold Svs.diff.
+    rewrite eval_varset_diff. destruct IHt1 as [_ IH1].
+    destruct q; [rewrite fmla_fv_fforalls | rewrite fmla_fv_fexists]; rewrite eval_varset_of_list, (IH1 _ He1);
+    reflexivity.
+  - (*Tbinop*) exfalso. apply (eval_binop_tm Heq Heval).
+  - (*Fbinop*) destruct (eval_binop_fmla Heq Heval) as [e1 [e2 [He [He1 He2]]]]. subst.
+    simpl. destruct IHt1 as [_ IH1]; destruct IHt2 as [_ IH2]. 
+    rewrite eval_varset_union, (IH1 _ He1), (IH2 _ He2); reflexivity.
+  - (*Tnot*) exfalso. apply (eval_not_tm Heq Heval).
+  - (*Fnot*) destruct (eval_not_fmla Heq Heval) as [e1 [He He1]]. subst. simpl. destruct_all; auto.
+  - (*Ttrue*) exfalso. apply (eval_true_tm Ht Heval).
+  - (*Ftrue*) rewrite (eval_true_fmla Ht Heval). reflexivity.
+  - (*Tfalse*) exfalso. apply (eval_false_tm Ht Heval).
+  - (*Ffalse*) rewrite (eval_false_fmla Ht Heval). reflexivity.
+Qed.
+
+Corollary t_free_vars_eval_term t e (Heval: eval_term t = Some e):
+  eval_varset (t_free_vars t) = tm_fv e.
+Proof.
+  apply t_free_vars_eval; auto.
+Qed.
+
+Corollary t_free_vars_eval_fmla t e (Heval: eval_fmla t = Some e): 
+  eval_varset (t_free_vars t) = fmla_fv e.
+Proof.
+  apply t_free_vars_eval; auto.
+Qed.
+
+(*[eval_varset] is invariant under mapping*)
+
+(*Could prove in general but whatever*)
+Lemma mvs_mem_map {A B: Type} (m: Mvs.t A) (f: A -> B) x:
+  Mvs.mem x (Mvs.map f m) = Mvs.mem x m.
+Proof.
+  rewrite !Mvs.mem_spec. destruct (Mvs.find_opt x m) as [y|] eqn : Hget1; simpl;
+  destruct (Mvs.find_opt x (Mvs.map f m)) as [y1|] eqn : Hget2; auto.
+  - assert (Hmem: Mvs.find_opt x (Mvs.map f m) = Some (f y)). {
+      apply Mvs.map_spec. exists x. exists y. split_all; auto. apply Vsym.Tg.eq_refl.
+    }
+    rewrite Hmem in Hget2; discriminate.
+  - rewrite Mvs.map_spec in Hget2. destruct Hget2 as [k1 [v1 [Heq [Hfind Hf]]]]; subst.
+    apply vsymbol_eqb_eq in Heq. subst. rewrite Hfind in Hget1. discriminate.
+Qed.
+
+Lemma eval_varset_map {A B: Type} (m: Mvs.t A) (f: A -> B):
+  eval_varset (Mvs.map f m) = eval_varset m.
+Proof.
+  apply aset_ext. intros x. rewrite !eval_varset_mem. setoid_rewrite mvs_mem_map. reflexivity.
+Qed.
+
 
 (*Now we can write a better eval_vsymbol function that is injective*)
 
@@ -1983,7 +2512,7 @@ Proof.
       destruct (eval_if_fmla Heq Heval) as [e2 [e3 [e4 [He1 [Heval1 [Heval2 Heval3]]]]]].
       subst. simpl. rewrite (IH1 _ Hm Hmty _ Heval1), (IH2' _ Hm Hmty _ Heval2), (IH3' _ Hm Hmty _ Heval3). reflexivity.
   - rewrite types_wf_rewrite, Heq in Hwf. (*TODO: add var condition*)
-    destruct Hwf as [Hwf1 Hwf2]. specialize (IHt1_1 Hwf1); specialize (IHt1_2 Hwf2). 
+    destruct Hwf as [Hvars [Hwf1 Hwf2]]. specialize (IHt1_1 Hwf1); specialize (IHt1_2 Hwf2). 
     destruct IHt1_1 as [IH1 _]; destruct IHt1_2 as [IH2 IH2'].
     split; intros m Hm Hmty e1 Heval.
     + (*tlet*) rewrite t_subst_unsafe_aux_rewrite, Heq. simpl.
@@ -1992,7 +2521,8 @@ Proof.
       rewrite (IH1 _ Hm Hmty _ Heval1). simpl. simpl in Heval2.
       (*Simplify the maps*)
       rewrite <- eval_subs_map_remove.
-      replace (tm_fv e3) with (eval_varset (bv_vars b)) by admit.
+      replace (tm_fv e3) with (eval_varset (bv_vars b)).
+      2: { erewrite <- eval_varset_map. rewrite Hvars. apply t_free_vars_eval_term. auto. }
       rewrite <- eval_subs_map_set_inter, eval_subs_map_is_empty.
       2: { eapply subs_map_submap; eauto. apply binding_submap. }
       destruct (amap_is_empty _).
@@ -2008,7 +2538,8 @@ Proof.
       rewrite (IH1 _ Hm Hmty _ Heval1). simpl. simpl in Heval2.
       (*Simplify the maps*)
       rewrite <- eval_subs_map_remove.
-      replace (fmla_fv e3) with (eval_varset (bv_vars b)) by admit.
+      replace (fmla_fv e3) with (eval_varset (bv_vars b)).
+      2: { erewrite <- eval_varset_map. rewrite Hvars. apply t_free_vars_eval_fmla. auto. }
       rewrite <- eval_subs_map_set_inter, eval_subs_map_is_empty.
       2: { eapply subs_map_submap; eauto. apply binding_submap. }
       destruct (amap_is_empty _).
@@ -2020,7 +2551,6 @@ Proof.
         -- eapply mvs_preserved; eauto. apply binding_submap.
   - (*Tcase*)
 
-  
 
 
       (*Need to prove these conditions equivalent - prove that
